new/golang/theory/proofmode.v
@@ -4,6 +4,7 @@ From Perennial.Helpers Require Export ipm.
 From iris.proofmode Require Import coq_tactics.
 (* make sure solve_proper comes from stdpp and not Coq *)
 From stdpp Require Export tactics.
+From New.golang.defn Require Export notation intoval.
 From New.golang.theory Require Export typing.
 From Perennial Require Export base.
 From Ltac2 Require Import Ltac2.
